coq/rfj.v
@@ -1,68 +1,50 @@
 Require Import Coq.Lists.List.
 Import ListNotations.
 
+Require Import Coq.Relations.Relation_Operators.
+
 Require Import MutualDistrust.fullabst.
 Require Import MutualDistrust.mutdist.
 
 (* Define RFJ interfaces *)
 
-Parameter rfj_class_declaration_table: Set.
-Parameter rfj_object_declaration_table: Set.
-Parameter rfj_cdt_domain: rfj_class_declaration_table -> list nat.
-
-Definition rfj_declaration_table: Set :=
-  (rfj_class_declaration_table * rfj_object_declaration_table)%type.
-
-Record rfj_interface: Set :=
-  {
-    rfj_interface_imports: rfj_declaration_table;
-    rfj_interface_exports: rfj_declaration_table
-  }.
-
+Parameter rfj_interface: Set.
 Parameter rfj_compatible2: rfj_interface -> rfj_interface -> Prop.
-
+(* Compatibility is pair-wise compatibility. *)
 Inductive rfj_compatible: list rfj_interface -> Prop :=
 | rfj_compatible_nil: rfj_compatible []
 | rfj_compatible_cons: forall C Cs,
                          rfj_compatible Cs ->
                          Forall (rfj_compatible2 C) Cs ->
                          rfj_compatible (C :: Cs).
-
 Parameter rfj_complete: list rfj_interface -> Prop.
+
+Lemma rfj_compatible_cons_inv:
+  forall I Is, rfj_compatible (I :: Is) -> rfj_compatible Is.
+Proof.
+  intros I Is H.
+  now inversion H.
+Qed.
 
 Instance rfji: interface_language rfj_interface :=
   {
     compatible := rfj_compatible;
+    compatible_cons := rfj_compatible_cons_inv;
     complete := rfj_complete
   }.
 
-(* Define RFJ *)
+(* Define RFJ as a component language *)
 
-Parameter rfj_class_definition_table: Set.
-Parameter rfj_object_definition_table: Set.
-
-Definition rfj_definition_table: Set :=
-  (rfj_class_definition_table * rfj_object_definition_table)%type.
-
-Parameter rfj_has_interface:
-  rfj_definition_table -> rfj_interface -> Prop.
-
-Record rfj_component: Type :=
-  {
-    rfj_component_interface: rfj_interface;
-    rfj_component_definitions: rfj_definition_table;
-    (* restrict to well-formed/well-typed components *)
-    rfj_component_wf:
-      rfj_has_interface rfj_component_definitions rfj_component_interface
-  }.
-
+Parameter rfj_defs: Set.
+Definition rfj_component: Set := (rfj_interface * rfj_defs)%type.
 Definition rfj_program := list rfj_component.
-
 Parameter rfj_beh_eq: rfj_program -> rfj_program -> Prop.
 
-Instance rfj : component_language rfji rfj_component rfj_program :=
+Parameter rfj_has_interface: rfj_defs -> rfj_interface -> Prop.
+
+Instance rfj: component_language rfji rfj_component rfj_program :=
   {
-    has_interface := fun C I => rfj_component_interface C = I;
+    has_interface := fun C I => fst C = I /\ rfj_has_interface (snd C) I;
     link := id;
     beh_eq := rfj_beh_eq
   }.
